@prefix : <http://www.bim4ren.eu/actors#> .
@prefix owl: <http://www.w3.org/2002/07/owl#> .
@prefix rdf: <http://www.w3.org/1999/02/22-rdf-syntax-ns#> .
@prefix xml: <http://www.w3.org/XML/1998/namespace> .
@prefix xsd: <http://www.w3.org/2001/XMLSchema#> .
@prefix rdfs: <http://www.w3.org/2000/01/rdf-schema#> .
@base <http://www.bim4ren.eu/actors> .

<http://www.bim4ren.eu/actors> rdf:type owl:Ontology ;
                                owl:versionIRI <http://www.bim4ren.eu/actors/0.1> .

#################################################################
#    Object Properties
#################################################################

###  http://www.bim4ren.eu/actors#ageCategory
:ageCategory rdf:type owl:ObjectProperty ;
             rdfs:domain :Actor ;
             rdfs:range :AgeCategory ;
             rdfs:comment "Relation describing the link between an actor and the corresponding age category"@fr ,
                          "Relation décrivant le lien entre un acteur et la catégorie d'âge correspondante"@fr ;
             rdfs:label "age category"@en ,
                        "catégorie d'âge"@fr .


###  http://www.bim4ren.eu/actors#associatedActor
:associatedActor rdf:type owl:ObjectProperty ;
                 rdfs:domain <https://w3id.org/bot#Zone> ;
                 rdfs:range :Actor ;
                 rdfs:comment "Relation describing the link between a zone and the associated actor, which could be the occupant or any actor having a specific role associated to the zone"@en ,
                              "Relation décrivant le lien entre une zone et un acteur associé, qui peut être l'occupant ou tout acteur ayant un rôle spécifique associé à cette zone"@fr ;
                 rdfs:label "acteur associé"@fr ,
                            "associated actor"@en .


###  http://www.bim4ren.eu/actors#associatedZone
:associatedZone rdf:type owl:ObjectProperty ;
                rdfs:range <https://w3id.org/bot#Zone> ;
                rdfs:comment "Relation pouvant décrire le lien entre un occupant et une zone associée à travers le profile d'occupation ou tout simplement le lien entre un acteur en général et une zone pour laquelle il a un role spécifique"@fr ,
                             "Relation that can describe the link between an occupant and an associated zone through the occupation profile or simply the link between an actor in general and a zone for which he has a specific role"@en ;
                rdfs:label "associated zone"@en ,
                           "zone associée"@fr .


###  http://www.bim4ren.eu/actors#hasEnergyPolicy
:hasEnergyPolicy rdf:type owl:ObjectProperty ;
                 rdfs:domain :Occupant ;
                 rdfs:range :EnergyPolicy ;
                 rdfs:comment "Property linking an occupant to the energy policy that he adopts"@en ,
                              "Propriété liant un occupant à la politique d'énergie qu'il adopte"@fr ;
                 rdfs:label "energy policy"@en ,
                            "politica energetica"@it ,
                            "politique énergétique"@fr ,
                            "política energética"@es .


###  http://www.bim4ren.eu/actors#occupancyProfile
:occupancyProfile rdf:type owl:ObjectProperty ;
                  rdfs:domain :Occupant ;
                  rdfs:range :OccupancyProfile ;
                  rdfs:comment "Relation describing the link between an occupant and its occupancy profile associated to a particular zone"@en ,
                               "Relation décrivant le lien entre un occupant et son profile d'occupation associé à une zone particulière"@fr ;
                  rdfs:label "occupancy profile"@fr ,
                             "profile d'occupation"@fr .


###  http://www.bim4ren.eu/actors#occupancyTime
:occupancyTime rdf:type owl:ObjectProperty ;
               rdfs:domain :OccupancyProfile ;
               rdfs:range :OccupancyTimeRange ;
               rdfs:comment "Relation describing the link between an occupancy profile (associated to an occupant and a given zone) and the corresponding occupancy time range"@en ,
                            "Relation décrivant le lien entre un profile d'occupation (associé à un occupant et une zone donnée) et l'intervalle d'occupation correspondant"@fr ;
               rdfs:label "occupancy time"@fr ,
                          "temps d'occupation"@en .


###  http://www.bim4ren.eu/actors#workSituation
:workSituation rdf:type owl:ObjectProperty ;
               rdfs:domain :Occupant ;
               rdfs:range :WorkSituation ;
               rdfs:comment "Relation describing the link between an occupant and its work situation"@en ,
                            "Relation décrivant le lien entre un occupant et la situation de travail correspondate"@fr ;
               rdfs:label "situation de travail"@fr ,
                          "work situation"@en .


###  http://www.bim4ren.eu/actors#workType
:workType rdf:type owl:ObjectProperty ;
          rdfs:domain :WorkSituation ;
          rdfs:range :WorkType ;
          rdfs:comment "Relation describing the link between a work situation associated to an occupant and the corresponding work type"@en ,
                       "Relation décrivant le lien entre la situation de travail associée à un occupant et le type de ce travail"@en ;
          rdfs:label "type de travail"@fr ,
                     "work type"@en .


#################################################################
#    Data properties
#################################################################

###  http://www.bim4ren.eu/actors#fromDateTime
:fromDateTime rdf:type owl:DatatypeProperty ;
              rdfs:range xsd:dateTime ;
              rdfs:comment "Property describing the start date and time related to an occupancy profile"@en ,
                           "Propriété décrivant la date et l'heure de début liées à un profil d'occupation"@fr ;
              rdfs:label "depuis date heure"@fr ,
                         "from date time"@en .


###  http://www.bim4ren.eu/actors#income
:income rdf:type owl:DatatypeProperty ;
        rdfs:range xsd:decimal ;
        rdfs:comment "Property describing the gross annual salary of an occupant"@en ,
                     "Propriété décrivant le salaire annuel brut d'un occupant"@fr ,
                     "salaire"@fr ;
        rdfs:label "income"@en .


###  http://www.bim4ren.eu/actors#toDateTime
:toDateTime rdf:type owl:DatatypeProperty ;
            rdfs:range xsd:dateTime ;
            rdfs:comment "Property describing the end date and time related to an occupancy profile"@en ,
                         "Propriété décrivant la date et l'heure de fin liées à un profil d'occupation"@fr ;
            rdfs:label "jusqu'au date heure"@fr ,
                       "to date time"@en .


#################################################################
#    Classes
#################################################################

###  http://www.bim4ren.eu/actors#Actor
:Actor rdf:type owl:Class ;
       rdfs:subClassOf [ rdf:type owl:Restriction ;
                         owl:onProperty :ageCategory ;
                         owl:maxQualifiedCardinality "1"^^xsd:nonNegativeInteger ;
                         owl:onClass :AgeCategory
                       ] ;
       rdfs:comment "A building actor, which comes down to a building manager, a building owner or an occupant"@en ,
                    "Un acteur du bâtiment, qui peut être un maître d'oeuvre, un maître d'ouvrage ou un occupant"@fr ;
       rdfs:isDefinedBy "http://bsdd.buildingsmart.org/#concept/details/3xQru0qRmHuO00025QrE$V"@en ;
       rdfs:label "Acteur"@fr ,
                  "Actor"@en .


###  http://www.bim4ren.eu/actors#AgeCategory
:AgeCategory rdf:type owl:Class ;
             rdfs:comment "Correspond à une classification selon les tranches d'ages de personnes"@fr ,
                          "Corresponds to a classification according to people age groups"@en ;
             rdfs:label "Age category"@en ,
                        "Catégorie d'âge"@fr .


###  http://www.bim4ren.eu/actors#BuildingManager
:BuildingManager rdf:type owl:Class ;
                 rdfs:subClassOf :Actor ;
                 owl:disjointWith :BuildingOwner ,
                                  :Occupant ;
                 rdfs:comment "Person or entity chosen by the building owner for the operational management of the work"@en ,
                              "Personne physique ou morale choisie par le maître d'ouvrage pour la conduite opérationnelle des travaux"@fr ;
                 rdfs:label "Building manager"@en ,
                            "Maître d'oeuvre"@fr .


###  http://www.bim4ren.eu/actors#BuildingOwner
:BuildingOwner rdf:type owl:Class ;
               rdfs:subClassOf :Actor ;
               rdfs:comment "Person or entity for whom the project is carried out"@en ,
                            "Personne physique ou morale pour laquelle le projet est réalisé"@fr ;
               rdfs:isDefinedBy "http://bsdd.buildingsmart.org/#concept/details/1B9uxpQzj5KBf25MREZyEH"@fr ;
               rdfs:label "Building owner"@en ,
                          "Maître d'ouvrage"@fr .


###  http://www.bim4ren.eu/actors#EnergyPolicy
:EnergyPolicy rdf:type owl:Class ;
              owl:equivalentClass [ rdf:type owl:Class ;
                                    owl:oneOf ( :COMFORT
                                                :ECO
                                                :ECO_PLUS
                                              )
                                  ] ;
              rdfs:comment "Defines to what extent the occupant pays attention to energy, and therefore has impacts on the heating or the use of certain devices during the simulation."@en ,
                           "Définit à quel point les occupants font attention ou non à l’énergie, et donc ont des impacts sur le chauffage ou l’utilisation de certains appareils durant la simulation. "@fr ;
              rdfs:label "Energy policy"@en ,
                         "Politica energetica"@it ,
                         "Politique énergétique"@fr ,
                         "Política energética"@es .


###  http://www.bim4ren.eu/actors#OccupancyProfile
:OccupancyProfile rdf:type owl:Class ;
                  rdfs:subClassOf [ rdf:type owl:Restriction ;
                                    owl:onProperty :occupancyTime ;
                                    owl:allValuesFrom :OccupancyTimeRange
                                  ] ,
                                  [ rdf:type owl:Restriction ;
                                    owl:onProperty :associatedZone ;
                                    owl:maxQualifiedCardinality "1"^^xsd:nonNegativeInteger ;
                                    owl:onClass <https://w3id.org/bot#Zone>
                                  ] ;
                  rdfs:comment "An occupancy profile describes some useful occupancy information (e.g., the occupancy time range) related to an occuppant associated to a given zone"@en ,
                               "Le profil d'occupation décrit certaines informations utiles (par exemple,les intervales d'occupation) liées à un occupant pour une zone donnée"@fr ;
                  rdfs:label "Occupancy profile"@en ,
                             "Profile d'occupation"@fr .


###  http://www.bim4ren.eu/actors#OccupancyTimeRange
:OccupancyTimeRange rdf:type owl:Class ;
                    rdfs:subClassOf [ rdf:type owl:Restriction ;
                                      owl:onProperty :fromDateTime ;
                                      owl:allValuesFrom xsd:dateTime
                                    ] ,
                                    [ rdf:type owl:Restriction ;
                                      owl:onProperty :toDateTime ;
                                      owl:allValuesFrom xsd:dateTime
                                    ] ;
                    rdfs:comment "L'intervalle de temps d'occupation lié à un occupant et une zone donnée"@fr ,
                                 "The occupancy time range related to an occupant and a given area"@en ;
                    rdfs:label "Intervalle de temps d'occupation"@fr ,
                               "Occupancy time range"@en .


###  http://www.bim4ren.eu/actors#Occupant
:Occupant rdf:type owl:Class ;
          rdfs:subClassOf :Actor ,
                          [ rdf:type owl:Restriction ;
                            owl:onProperty :occupancyProfile ;
                            owl:allValuesFrom :OccupancyProfile
                          ] ,
                          [ rdf:type owl:Restriction ;
                            owl:onProperty :workSituation ;
                            owl:allValuesFrom :WorkSituation
                          ] ;
          rdfs:comment "A type of actor that defines the form of occupancy of a property"@en ,
                       "Un type d'acteur qui définit la forme d'occupation d'une propriété"@fr ;
          rdfs:isDefinedBy "http://bsdd.buildingsmart.org/#concept/details/289KpOp8L4MBqIToXk2Uxq"@en ;
          rdfs:label "Occupant"@en ,
                     "Occupant"@fr .


###  http://www.bim4ren.eu/actors#WorkSituation
:WorkSituation rdf:type owl:Class ;
               rdfs:subClassOf [ rdf:type owl:Restriction ;
                                 owl:onProperty :workType ;
                                 owl:allValuesFrom :WorkType
                               ] ,
                               [ rdf:type owl:Restriction ;
                                 owl:onProperty :income ;
                                 owl:allValuesFrom xsd:decimal
                               ] ;
               rdfs:comment "Describes the work situation of an occupant, mainly the type of work (if any), and its related income"@en ,
                            "Décrit la situation de travail d'un occupant, principalement le type de travail (le cas échéant) et son revenu"@fr ;
               rdfs:label "Situation de travail"@fr ,
                          "Work situation"@en .


###  http://www.bim4ren.eu/actors#WorkType
:WorkType rdf:type owl:Class ;
          owl:equivalentClass [ rdf:type owl:Class ;
                                owl:oneOf ( :EMPLOYED
                                            :SELF_EMPLOYED
                                            :UNEMPLOYED
                                          )
                              ] ;
          rdfs:comment "Describes the occupant type of work"@en ,
                       "Décrit le type de travail d'un occupant"@fr ;
          rdfs:label "Type de travail"@fr ,
                     "Work type"@en .


###  https://w3id.org/bot#Zone
<https://w3id.org/bot#Zone> rdf:type owl:Class .


#################################################################
#    Individuals
#################################################################

###  http://www.bim4ren.eu/actors#ADULT
:ADULT rdf:type owl:NamedIndividual ,
                :AgeCategory ;
       rdfs:comment "An adult is a person aged between 18 and 64 inclusive"@en ,
                    "Un adulte est une personne âgée antre 18 et 64 ans inclus"@fr ;
       rdfs:label "Adult"@en ,
                  "Adulte"@fr .


###  http://www.bim4ren.eu/actors#BABY
:BABY rdf:type owl:NamedIndividual ,
               :AgeCategory ;
      rdfs:comment "A baby is a person who is less than a year old"@en ,
                   "Un bébé est une personne qui a moins d'un an"@fr ;
      rdfs:label "Baby"@en ,
                 "Bébé"@fr .


###  http://www.bim4ren.eu/actors#CHILD
:CHILD rdf:type owl:NamedIndividual ,
                :AgeCategory ;
       rdfs:comment "A child is a person aged between 1 year and 11 years inclusive"@en ,
                    "Un enfant est une personne âgée entre 1 an et 11 ans inclus"@fr ;
       rdfs:label "Child"@en ,
                  "Enfant"@fr .


###  http://www.bim4ren.eu/actors#COMFORT
:COMFORT rdf:type owl:NamedIndividual ,
                  :EnergyPolicy ;
         rdfs:comment "An occupant who is not eco friendly"@en ,
                      "Un occupant qui n'est pas éco-responsable"@fr ;
         rdfs:label "Comfort"@en ,
                    "Comodidad"@es ,
                    "Comodità"@it ,
                    "Confort"@fr .


###  http://www.bim4ren.eu/actors#ECO
:ECO rdf:type owl:NamedIndividual ,
              :EnergyPolicy ;
     rdfs:comment "An occupant who is eco friendly"@en ,
                  "Un occupant éco-responsable"@fr ;
     rdfs:label "Eco friendly"@en ,
                "Eco-responsable"@fr ,
                "Ecológico"@es ,
                "Ecológico"@it .


###  http://www.bim4ren.eu/actors#ECO_PLUS
:ECO_PLUS rdf:type owl:NamedIndividual ,
                   :EnergyPolicy ;
          rdfs:comment "An occupant who is eco friendly++"@en ,
                       "Un occupant éco-responsable++"@fr ;
          rdfs:label "Eco friendly++"@en ,
                     "Eco-responsable++"@fr ,
                     "Ecológico++"@es ,
                     "Ecológico++"@it .


###  http://www.bim4ren.eu/actors#ELDERLY
:ELDERLY rdf:type owl:NamedIndividual ,
                  :AgeCategory ;
         rdfs:comment "An elderly is a person aged 65 and over"@en ,
                      "Un personne âgée est une personne qui a 65 ans et plus"@fr ;
         rdfs:label "Elderly"@en ,
                    "Personne âgée"@fr .


###  http://www.bim4ren.eu/actors#EMPLOYED
:EMPLOYED rdf:type owl:NamedIndividual ,
                   :WorkType ;
          rdfs:comment "An occupant having a paid job"@en ,
                       "Un occupant ayant un emploi rémunéré"@fr ;
          rdfs:label "Employed"@en ,
                     "Employé"@fr .


###  http://www.bim4ren.eu/actors#SELF_EMPLOYED
:SELF_EMPLOYED rdf:type owl:NamedIndividual ,
                        :WorkType ;
               rdfs:comment "An occupant who is working for oneself as a freelance or who is the owner of a business"@en ,
                            "Un occupant qui travaille pour soi-même en tant que freelance ou qui est le propriétaire d'une entreprise"@fr ;
               rdfs:label "Self employed"@en ,
                          "Travailleur indépendant"@fr .


###  http://www.bim4ren.eu/actors#TEENAGER
:TEENAGER rdf:type owl:NamedIndividual ,
                   :AgeCategory ;
          rdfs:comment "A teenager is a person aged between 12 and 17 years inclusive"@en ,
                       "Un adolescent est une personne âgée entre 12 et 17 ans inclus"@fr ;
          rdfs:label "Adolescent"@fr ,
                     "Teenager"@en .


###  http://www.bim4ren.eu/actors#UNEMPLOYED
:UNEMPLOYED rdf:type owl:NamedIndividual ,
                     :WorkType ;
            rdfs:comment "An occupant without a paid job"@en ,
                         "Un occupant sans emploi"@fr ;
            rdfs:label "Unemployed"@en ,
                       "sans emploi"@fr .


###  Generated by the OWL API (version 5.1.14) https://github.com/owlcs/owlapi/
