@prefix : <https://w3id.org/dot#> .
@prefix owl: <http://www.w3.org/2002/07/owl#> .
@prefix rdf: <http://www.w3.org/1999/02/22-rdf-syntax-ns#> .
@prefix xml: <http://www.w3.org/XML/1998/namespace> .
@prefix xsd: <http://www.w3.org/2001/XMLSchema#> .
@prefix rdfs: <http://www.w3.org/2000/01/rdf-schema#> .
@base <https://w3id.org/dot#> .

<https://w3id.org/dot#> rdf:type owl:Ontology ;
                         owl:versionIRI <https://w3id.org/dot/0.8> ;
                         <http://purl.org/dc/terms/contributor> _:genid1 ;
                         <http://purl.org/dc/terms/creator> <https://www.researchgate.net/profile/Mathias_Bonduel> ,
                                                            _:genid2 ;
                         <http://purl.org/dc/terms/issued> "2018-10-12"^^xsd:date ;
                         <http://purl.org/dc/terms/license> "https://creativecommons.org/licenses/by/1.0" ;
                         <http://purl.org/dc/terms/modified> "2019-02-17"^^xsd:date ;
                         <http://purl.org/dc/terms/title> "Damage Topology Ontology"@en ;
                         <http://purl.org/vocab/vann/example> "https://madsholten.github.io/sparql-visualizer/?file=https://raw.githubusercontent.com/Alhakam/dot/master/ABox-Examples/dot-demo.json"^^xsd:anyURI ,
                                                              "https://raw.githubusercontent.com/Alhakam/dot/master/ABox-Examples/dotSampleData_pt1.ttl"^^xsd:anyURI ,
                                                              "https://raw.githubusercontent.com/Alhakam/dot/master/ABox-Examples/dotSampleData_pt2.ttl"^^xsd:anyURI ;
                         <http://purl.org/vocab/vann/preferredNamespacePrefix> "dot" ;
                         <http://purl.org/vocab/vann/preferredNamespaceUri> "https://w3id.org/dot#" ;
                         rdfs:comment """- Version 0.8: 
* completed ontology metadata wrt LOV
* added classes dot:ClassifiedDamage and dot:UnclassifiedDamage (subclasses of dot:Damage)
* made dot:StructuralDamage and dot:Defect subclasses of dot:Damage
"""@en ;
                         owl:versionInfo "0.8" .

_:genid1 rdf:type <http://xmlns.com/foaf/0.1/Person> ;
          <http://xmlns.com/foaf/0.1/name> "Mads Holten Rasmussen" .

_:genid2 rdf:type <http://xmlns.com/foaf/0.1/Person> ;
          <http://xmlns.com/foaf/0.1/name> "Al-Hakam Hamdan" .

#################################################################
#    Annotation properties
#################################################################

###  http://purl.org/dc/terms/contributor
<http://purl.org/dc/terms/contributor> rdf:type owl:AnnotationProperty .


###  http://purl.org/dc/terms/creator
<http://purl.org/dc/terms/creator> rdf:type owl:AnnotationProperty .


###  http://purl.org/dc/terms/issued
<http://purl.org/dc/terms/issued> rdf:type owl:AnnotationProperty .


###  http://purl.org/dc/terms/license
<http://purl.org/dc/terms/license> rdf:type owl:AnnotationProperty .


###  http://purl.org/dc/terms/modified
<http://purl.org/dc/terms/modified> rdf:type owl:AnnotationProperty .


###  http://purl.org/dc/terms/title
<http://purl.org/dc/terms/title> rdf:type owl:AnnotationProperty .


###  http://purl.org/vocab/vann/example
<http://purl.org/vocab/vann/example> rdf:type owl:AnnotationProperty .


###  http://purl.org/vocab/vann/preferredNamespacePrefix
<http://purl.org/vocab/vann/preferredNamespacePrefix> rdf:type owl:AnnotationProperty .


###  http://purl.org/vocab/vann/preferredNamespaceUri
<http://purl.org/vocab/vann/preferredNamespaceUri> rdf:type owl:AnnotationProperty .


###  http://schema.org/#domainIncludes
<http://schema.org/#domainIncludes> rdf:type owl:AnnotationProperty .


###  http://xmlns.com/foaf/0.1/name
<http://xmlns.com/foaf/0.1/name> rdf:type owl:AnnotationProperty .


#################################################################
#    Object Properties
#################################################################

###  https://w3id.org/dot#adjacentDamageElement
:adjacentDamageElement rdf:type owl:ObjectProperty ,
                                owl:SymmetricProperty ;
                       rdfs:domain :DamageElement ;
                       rdfs:range :DamageElement ;
                       rdfs:comment "Definerer relationen mellem to Skadeselementer som er fysisk forbundet til hinanden."@da ,
                                    "Defines the relationship between two instances of DamageElement that are physically connected with each other."@en ;
                       rdfs:isDefinedBy <https://w3id.org/dot#> ;
                       rdfs:label "adjacent DamageElement"@en ,
                                  "tilstødende Skadeselement"@da .


###  https://w3id.org/dot#aggregatesDamageElement
:aggregatesDamageElement rdf:type owl:ObjectProperty ;
                         rdfs:domain :DamageArea ;
                         rdfs:range :DamageElement ;
                         owl:propertyChainAxiom ( :aggregatesDamageElement
                                                  :adjacentDamageElement
                                                ) ,
                                                ( :aggregatesDamagePattern
                                                  :groupsDamageElement
                                                ) ;
                         rdfs:comment "A relationship between an instance of Damage Area and its consisting DamageElement instance."@en ,
                                      "En relation mellem et Skadeselement og det eller de Skadesområder som dette udgøres af."@da ;
                         rdfs:isDefinedBy <https://w3id.org/dot#> ;
                         rdfs:label "aggregates Damage Element"@en ,
                                    "aggregerer Skadeselement"@da .


###  https://w3id.org/dot#aggregatesDamagePattern
:aggregatesDamagePattern rdf:type owl:ObjectProperty ;
                         rdfs:domain :DamageArea ;
                         rdfs:range :DamagePattern ;
                         rdfs:comment "A relationship between an instance of DamageArea and its consisting DamagePattern instance."@en ,
                                      "En relation mellem et Skadesområde og det eller de Skademønstre som dette udgøres af."@da ;
                         rdfs:isDefinedBy <https://w3id.org/dot#> ;
                         rdfs:label "aggregates Damage Pattern"@en ,
                                    "aggregerer Skademønster"@da .


###  https://w3id.org/dot#coveredByInspection
:coveredByInspection rdf:type owl:ObjectProperty ;
                     rdfs:range :Inspection ;
                     owl:propertyChainAxiom ( :coveredInDocumentation
                                              :documentationFromInspection
                                            ) ;
                     <http://schema.org/#domainIncludes> <https://w3id.org/bot#Element> ,
                                                         <https://w3id.org/bot#Zone> ,
                                                         :Damage ,
                                                         <https://wisib.de/ontologie/brot#BridgeElement> ,
                                                         <https://wisib.de/ontologie/brot#BridgeSpatialZone> ;
                     rdfs:comment "Relation mellem et dokumenteret objekt (skade eller komponent / zone) og Inspektionen hvoraf objektet er omfattet."@da ,
                                  "Relationship between a documented object (damage or component / zone) and the Inspection in which the object has been covered."@en ;
                     rdfs:isDefinedBy <https://w3id.org/dot#> ;
                     rdfs:label "covered by inspection"@en ,
                                "omfattet af inspektion"@da .


###  https://w3id.org/dot#coveredInDocumentation
:coveredInDocumentation rdf:type owl:ObjectProperty ;
                        rdfs:range :Documentation ;
                        <http://schema.org/#domainIncludes> <https://w3id.org/bot#Element> ,
                                                            <https://w3id.org/bot#Zone> ,
                                                            :Damage ,
                                                            <https://wisib.de/ontologie/brot#BridgeElement> ,
                                                            <https://wisib.de/ontologie/brot#BridgeSpatialZone> ;
                        rdfs:comment "Relation mellem en Dokumentation og det relevante dokumenterede eller inspicerede objekt (fx dot:DamageArea eller bot:Element). Bør kun benyttes for skadesrelevant dokumentation."@da ,
                                     "Relationship between a Documentation and the relevant documented or inspected object (e.g. dot:DamageArea or bot:Element). Should only be used for damage-relevant documentations."@en ;
                        rdfs:isDefinedBy <https://w3id.org/dot#> ;
                        rdfs:label "covered by documentation"@en ,
                                   "omfattet af dokumentation"@da .


###  https://w3id.org/dot#documentationFromInspection
:documentationFromInspection rdf:type owl:ObjectProperty ;
                             rdfs:comment "Relation mellem en Dokumentation og Inspektionen som Dokumentationen refererer til. Omvendt objektegenskab af dot:hasDocumentation."@da ,
                                          "Relationship between a Documentation and the Inspection to which the Documentation refers. Inverse object property of dot:hasDocumentation."@en ;
                             rdfs:isDefinedBy <https://w3id.org/dot#> ;
                             rdfs:label "documentation from inspection"@en ,
                                        "dokumentation fra inspektion"@da .


###  https://w3id.org/dot#groupsDamageElement
:groupsDamageElement rdf:type owl:ObjectProperty ;
                     rdfs:domain :DamagePattern ;
                     rdfs:range :DamageElement ;
                     owl:propertyChainAxiom ( :groupsDamageElement
                                              :adjacentDamageElement
                                            ) ;
                     rdfs:comment "Groups instances of DamageElement that are physically connected in a DamagePattern."@en ,
                                  "Grupperer Skadeelementer som er fysisk forbundet i et Skademønster."@da ;
                     rdfs:isDefinedBy <https://w3id.org/dot#> ;
                     rdfs:label "groups Damage Elements"@en ,
                                "grupperer Skadeelement"@da .


###  https://w3id.org/dot#hasCausation
:hasCausation rdf:type owl:ObjectProperty ;
              rdfs:domain :Damage ;
              rdfs:range :Causation ;
              rdfs:comment "Relation mellem en Skade og dens Forårsagelse."@da ,
                           "Relationship between a Damage and its Causation."@en ;
              rdfs:isDefinedBy <https://w3id.org/dot#> ;
              rdfs:label "har Forårsagelse"@da ,
                         "has Causation"@en .


###  https://w3id.org/dot#hasDamage
:hasDamage rdf:type owl:ObjectProperty ;
           rdfs:range :Damage ;
           <http://schema.org/#domainIncludes> <https://w3id.org/bot#Element> ,
                                               <https://w3id.org/bot#Zone> ,
                                               <https://wisib.de/ontologie/brot#BridgeElement> ,
                                               <https://wisib.de/ontologie/brot#BridgeSpatialZone> ;
           rdfs:comment "Definerer relationen mellem en påvirket bygningsdel eller konstruktion (fx bot:Element) og en Skade."@da ,
                        "Defines the relationship between an affected component or structure (e.g. bot:Element) and a Damage."@en ;
           rdfs:isDefinedBy <https://w3id.org/dot#> ;
           rdfs:label "har Skade"@da ,
                      "has Damage"@en .


###  https://w3id.org/dot#hasDamageArea
:hasDamageArea rdf:type owl:ObjectProperty ;
               rdfs:subPropertyOf :hasDamage ;
               rdfs:range :DamageArea ;
               rdfs:comment "Definerer relationen mellem en påvirket bygningsdel eller konstruktion (fx bot:Element) og et Skadesområde."@da ,
                            "Defines the relationship between an affected component or structure (e.g. bot:Element) and a DamageArea."@en ;
               rdfs:isDefinedBy <https://w3id.org/dot#> ;
               rdfs:label "har Skadesområde"@da ,
                          "has DamageArea"@en .


###  https://w3id.org/dot#hasDamageElement
:hasDamageElement rdf:type owl:ObjectProperty ;
                  rdfs:subPropertyOf :hasDamage ;
                  rdfs:range :DamageElement ;
                  owl:propertyChainAxiom ( :hasDamageArea
                                           :aggregatesDamageElement
                                         ) ;
                  rdfs:comment "Definerer relationen mellem en påvirket bygningsdel eller konstruktion (fx bot:Element) og et Skadeselement."@da ,
                               "Defines the relationship between an affected component or structure (e.g. bot:Element) and a DamageElement."@en ;
                  rdfs:isDefinedBy <https://w3id.org/dot#> ;
                  rdfs:label "har Skadeselement"@da ,
                             "has DamageElement"@en .


###  https://w3id.org/dot#hasDocumentation
:hasDocumentation rdf:type owl:ObjectProperty ;
                  owl:inverseOf :documentationFromInspection ;
                  rdfs:domain :Inspection ;
                  rdfs:range :Documentation ;
                  rdfs:comment "Relation mellem en Inspektion den tilhørende Dokumentation."@da ,
                               "Relationship between an Inspection and the corresponding Documentation"@en ;
                  rdfs:isDefinedBy <https://w3id.org/dot#> ;
                  rdfs:label "har dokumentation"@da ,
                             "has documentation"@en .


###  https://w3id.org/dot#hasInspector
:hasInspector rdf:type owl:ObjectProperty ;
              rdfs:domain :Inspection ;
              rdfs:range :Inspector ;
              rdfs:comment "Relation mellem en Inspektør og en Inspektion udført af denne person."@da ,
                           "Relationship between an Inspector and the Inspection that has been performed by him."@en ;
              rdfs:isDefinedBy <https://w3id.org/dot#> ;
              rdfs:label "har Inspektør"@da ,
                         "has Inspector"@en .


#################################################################
#    Data properties
#################################################################

###  http://purl.org/dc/terms/description
<http://purl.org/dc/terms/description> rdf:type owl:DatatypeProperty .


###  https://w3id.org/dot#descriptionContent
:descriptionContent rdf:type owl:DatatypeProperty ;
                    rdfs:subPropertyOf <http://purl.org/dc/terms/description> ;
                    rdfs:domain :Description ;
                    rdfs:range xsd:string ;
                    rdfs:comment "Tekstbeskrivelse om en konstruktionsdel eller skade."@da ,
                                 "Textual content used for the Description of a Structure Element or Damage."@en ;
                    rdfs:isDefinedBy <https://w3id.org/dot#> ;
                    rdfs:label "beskrivelseskontekst"@da ,
                               "description content"@en .


###  https://w3id.org/dot#filePath
:filePath rdf:type owl:DatatypeProperty ;
          rdfs:domain :ExternalResource ;
          rdfs:range xsd:anyURI ;
          rdfs:comment "Definerer en ekstern resources unikke sti i et filsystem."@da ,
                       "Defines the unique location in a file system of an ExternalResource."@en ;
          rdfs:isDefinedBy <https://w3id.org/dot#> ;
          rdfs:label "file path"@en ,
                     "filsti"@da .


#################################################################
#    Classes
#################################################################

###  http://purl.org/vocommons/voaf#Vocabulary
<http://purl.org/vocommons/voaf#Vocabulary> rdf:type owl:Class .


###  http://xmlns.com/foaf/0.1/Person
<http://xmlns.com/foaf/0.1/Person> rdf:type owl:Class .


###  https://w3id.org/dot#Causation
:Causation rdf:type owl:Class ;
           rdfs:comment """Represents the causation of a damage.
Should be extended with domain-specific subclasses."""@en ,
                        """Repræsenterer skadens forårsagelse. 
Bør specificeres af en domæne-specifik underklasse."""@da ;
           rdfs:isDefinedBy <https://w3id.org/dot#> ;
           rdfs:label "Causation"@en ,
                      "Forårsagelse"@da .


###  https://w3id.org/dot#ClassifiedDamage
:ClassifiedDamage rdf:type owl:Class ;
                  rdfs:subClassOf :Damage ;
                  owl:disjointWith :UnclassifiedDamage ;
                  rdfs:comment """A damage classification is used to denote the kind of damage. Subclasses of this class are defined in extensions 
			  such as CDO (Concrete Damage Ontology), NSO (the Natural Stone Ontology), etc."""@en ;
                  rdfs:isDefinedBy <https://w3id.org/dot#> ;
                  rdfs:label "Classified Damage"@en .


###  https://w3id.org/dot#Damage
:Damage rdf:type owl:Class ;
        rdfs:comment """Damage is the harm to a structure resulting in impairment or loss of function, usefulness or value.
Instead of using dot:Damage, it is recommended to use one subclass of dot:Damage for respectively the damage topology (either dot:DamageArea or dot:DamageElement), the 
potential structural impact (either dot:StructuralDamage or dot:Defect) and the damage classification (either dot:UnclassifiedDamage or subclasses of dot:ClassifiedDamage)."""@en ,
                     """En Skade er en beskadigelse af en konstruktion, der resulterer i forringelse eller tab af funktion, nyttighed eller værdi.
I stedet for at benytte dot:Damage anbefales det at bruge en af underklasserne (enten dot:DamageArea eller dot:DamageElement)."""@da ;
        rdfs:isDefinedBy <https://w3id.org/dot#> ;
        rdfs:label "Damage"@en ,
                   "Skade"@da .


###  https://w3id.org/dot#DamageArea
:DamageArea rdf:type owl:Class ;
            rdfs:subClassOf :Damage ;
            owl:disjointWith :DamageElement ,
                             :DamagePattern ;
            rdfs:comment "Area in a component where damage is located. Holds collection of multiple DamageElements or DamagePatterns. Used to be attached with simplified geometry."@en ,
                         "Område i et objekt hvor der er en beskadigelse. Beskriver en samling af et eller flere Skadeselementer eller Skadesmønstre. Kan tilknyttes simplificeret geometri."@da ;
            rdfs:isDefinedBy <https://w3id.org/dot#> ;
            rdfs:label "Damage Area"@en ,
                       "Skadesområde"@da .


###  https://w3id.org/dot#DamageElement
:DamageElement rdf:type owl:Class ;
               rdfs:subClassOf :Damage ;
               owl:disjointWith :DamagePattern ;
               rdfs:comment "Damage that is modeled on a very detailed level and belongs with other adjacent Damage Element instances to a broader damage area or damage pattern"@en ,
                            "En skade som er modelleret på et detaljeret niveau og hører sammen med andre tilstødende Skadeselementer i et større Skadesområde eller Skadesmønster."@da ;
               rdfs:isDefinedBy <https://w3id.org/dot#> ;
               rdfs:label "Damage Element"@en ,
                          "Skadeselement"@da .


###  https://w3id.org/dot#DamagePattern
:DamagePattern rdf:type owl:Class ;
               rdfs:comment "Definerer en gruppe af assosierede eller fysisk forbundne Skadesområder. Benyttes til at gruppere Skadesområder."@da ,
                            "Defines a group of associated or physically connected instances of DamageElement. Used as class for grouping inside an instance of DamageArea."@en ;
               rdfs:isDefinedBy <https://w3id.org/dot#> ;
               rdfs:label "Damage Pattern"@en ,
                          "Skadesmønster"@da .


###  https://w3id.org/dot#Defect
:Defect rdf:type owl:Class ;
        rdfs:subClassOf :Damage ;
        owl:disjointWith :StructuralDamage ;
        rdfs:comment """Benyttes på ting der allerede er klassificeret som et dot:DamageArea, dot:DamagePattern eller dot:DamageElement.
En Skade der ikke svækker den konstruktionsmæssige bæreevne, men som stadig har en indflydelse på holdbarheden, brugbarheden og / eller værdien."""@da ,
                     """Should be used on nodes that are already classified as dot:DamageArea or dot:DamageElement.
Damage that does not impair the structural integrity of the structure, but can still have influence on the durability, usability and / or value."""@en ;
        rdfs:isDefinedBy <https://w3id.org/dot#> ;
        rdfs:label "Defect"@en ,
                   "Defekt"@da .


###  https://w3id.org/dot#Description
:Description rdf:type owl:Class ;
             rdfs:subClassOf :Documentation ;
             rdfs:comment "Kort tekstbeskrivelse om en Skade eller Konstruktionsdel. Typisk opretted af Inspektøren."@da ,
                          "Short textual documentation about a Damage or Structure Element. Generally created by the inspecting person."@en ;
             rdfs:isDefinedBy <https://w3id.org/dot#> ;
             rdfs:label "Beskrivelse"@da ,
                        "Description"@en .


###  https://w3id.org/dot#Documentation
:Documentation rdf:type owl:Class ;
               rdfs:comment "Material or data that provides information or evidence about the structure and its components or that serves as a record. Should only be used for damage-related documentation."@en ,
                            "Materiale eller data der tilvejebringer information eller bevis om konstruktionen og dens bestanddele eller som fungerer som journal. Bør kun benyttes for skadesrelateret dokumentation."@da ;
               rdfs:isDefinedBy <https://w3id.org/dot#> ;
               rdfs:label "Damage Documentation"@en ,
                          "Skadesdokumentation"@da .


###  https://w3id.org/dot#ExternalResource
:ExternalResource rdf:type owl:Class ;
                  rdfs:subClassOf :Documentation ;
                  rdfs:comment "Document that is stored in a separate file, referenced by an external path."@en ,
                               "Dokument der gemmes i en seperat fil, refereret af en ekstern sti."@da ;
                  rdfs:isDefinedBy <https://w3id.org/dot#> ;
                  rdfs:label "Ekstern Resource"@da ,
                             "External Resource"@en .


###  https://w3id.org/dot#Inspection
:Inspection rdf:type owl:Class ;
            rdfs:comment """Careful examination or scrutiny in which an existing construction or a part of it is inspected and detected damages are recorded.
Should be repeated at regular time intervals."""@en ,
                         """Omhyggelig undersøgelse eller granskning hvori en eksisterende konstruktion eller en del ad denne inspiceres og detekterede beskadigelser registreres.
Inspektioner bør udføres regelmæssigt."""@da ;
            rdfs:isDefinedBy <https://w3id.org/dot#> ;
            rdfs:label "Inspection"@en ,
                       "Inspektion"@da .


###  https://w3id.org/dot#Inspector
:Inspector rdf:type owl:Class ;
           rdfs:subClassOf <http://xmlns.com/foaf/0.1/Person> ;
           rdfs:comment "A person who inspects constructions (for damages) or whose task it is to carry out inspections on constructions."@en ,
                        "En person der inspicerer konstruktioner (for skader) eller hvis opgave er at udføre inspektioner af konstruktioner."@da ;
           rdfs:isDefinedBy <https://w3id.org/dot#> ;
           rdfs:label "Inspector"@en ,
                      "Inspektør"@da .


###  https://w3id.org/dot#StructuralDamage
:StructuralDamage rdf:type owl:Class ;
                  rdfs:subClassOf :Damage ;
                  rdfs:comment """Benyttes på ting der allerede er klassificeret som et dot:DamageArea, dot:DamagePattern eller dot:DamageElement.
En Skade der svækker den konstruktionsmæssige bæreevne."""@da ,
                               """Should be used on nodes that are already classified as dot:DamageArea, dot:DamagePattern or dot:DamageElement.
Damage that impairs the structural integrity of the structure."""@en ;
                  rdfs:isDefinedBy <https://w3id.org/dot#> ;
                  rdfs:label "Konstruktionsmæssig Skade"@da ,
                             "Structural Damage"@en .


###  https://w3id.org/dot#UnclassifiedDamage
:UnclassifiedDamage rdf:type owl:Class ;
                    rdfs:subClassOf :Damage ;
                    rdfs:comment """A dot:Damage instance that is not further classified with domain-specific classes (subclasses of dot:ClassifiedDamage). 
This class can be used in cases where the damage classification is unknown."""@en ;
                    rdfs:isDefinedBy <https://w3id.org/dot#> ;
                    rdfs:label "Unclassified Damage"@en .


#################################################################
#    Individuals
#################################################################

###  https://w3id.org/dot#
<https://w3id.org/dot#> rdf:type owl:NamedIndividual ,
                                 <http://purl.org/vocommons/voaf#Vocabulary> ;
                        <http://purl.org/dc/terms/description> "Ontology that defines the topology of damages in constructions."@en .


###  Generated by the OWL API (version 5.1.14) https://github.com/owlcs/owlapi/
